pico-invsubtyping-limitedvpa/Properties.v
@@ -1041,7 +1041,7 @@ Proof.
 Qed.
 
 Lemma eval_stmt_preserves_heap_domain_simple : forall CT rΓ h stmt rΓ' h',
-  eval_stmt OK CT rΓ h stmt OK rΓ' h' ->
+  eval_stmt OK (protected_locset_from_env CT h rΓ) CT rΓ h stmt OK (protected_locset_from_env CT h rΓ) rΓ' h' ->
   dom h <= dom h'.
 Proof.
   intros CT rΓ h stmt rΓ' h' Heval.
@@ -1081,7 +1081,7 @@ Qed.
 (* Not just length, there is no statement can do strong update. *)
 Lemma eval_stmt_preserves_r_type : 
   forall CT rΓ h stmt rΓ' h' loc rqt,
-    eval_stmt OK CT rΓ h stmt OK rΓ' h' ->
+    eval_stmt OK (protected_locset_from_env CT h rΓ) CT rΓ h stmt OK (protected_locset_from_env CT h rΓ) rΓ' h' ->
     r_type h loc = Some rqt ->
     loc < dom h ->
     r_type h' loc = Some rqt.
@@ -1129,7 +1129,7 @@ Qed.
 
 Lemma eval_stmt_preserves_r_muttype : 
   forall CT rΓ h stmt rΓ' h' loc q,
-    eval_stmt OK CT rΓ h stmt OK rΓ' h' ->
+    eval_stmt OK (protected_locset_from_env CT h rΓ) CT rΓ h stmt OK (protected_locset_from_env CT h rΓ) rΓ' h' ->
     r_muttype h loc = Some q ->
     loc < dom h ->
     r_muttype h' loc = Some q.
@@ -1505,7 +1505,7 @@ Qed.
 Lemma eval_stmt_preserves_receiver_addr_typed :
   forall CT sΓ rΓ h stmt sΓ' rΓ' h' ι,
     stmt_typing CT sΓ stmt sΓ' ->
-    eval_stmt OK CT rΓ h stmt OK rΓ' h' ->
+    eval_stmt OK (protected_locset_from_env CT h rΓ) CT rΓ h stmt OK (protected_locset_from_env CT h rΓ) rΓ' h' ->
     get_this_var_mapping (vars rΓ) = Some ι ->
     get_this_var_mapping (vars rΓ') = Some ι.
 Proof.
@@ -1578,7 +1578,7 @@ Lemma eval_stmt_preserves_receiver_addr_typed_backwards :
   forall CT sΓ rΓ h stmt sΓ' rΓ' h' ι,
     wf_r_config CT sΓ rΓ h ->
     stmt_typing CT sΓ stmt sΓ' ->
-    eval_stmt OK CT rΓ h stmt OK rΓ' h' ->
+    eval_stmt OK (protected_locset_from_env CT h rΓ) CT rΓ h stmt OK (protected_locset_from_env CT h rΓ) rΓ' h' ->
     get_this_var_mapping (vars rΓ') = Some ι ->
     get_this_var_mapping (vars rΓ) = Some ι.
 Proof.
@@ -1609,7 +1609,7 @@ Lemma eval_stmt_preserves_receiver_addr_mapping_eq :
   forall CT sΓ rΓ h stmt sΓ' rΓ' h',
     wf_r_config CT sΓ rΓ h ->
     stmt_typing CT sΓ stmt sΓ' ->
-    eval_stmt OK CT rΓ h stmt OK rΓ' h' ->
+    eval_stmt OK (protected_locset_from_env CT h rΓ) CT rΓ h stmt OK (protected_locset_from_env CT h rΓ) rΓ' h' ->
     get_this_var_mapping (vars rΓ) =
     get_this_var_mapping (vars rΓ').
 Proof.
@@ -1638,7 +1638,7 @@ Corollary eval_stmt_preserves_receiver_addr_eq_loc' :
   forall CT sΓ rΓ h stmt sΓ' rΓ' h' ι1 ι2,
     wf_r_config CT sΓ rΓ h ->
     stmt_typing CT sΓ stmt sΓ' ->
-    eval_stmt OK CT rΓ h stmt OK rΓ' h' ->
+    eval_stmt OK (protected_locset_from_env CT h rΓ) CT rΓ h stmt OK (protected_locset_from_env CT h rΓ) rΓ' h' ->
     get_this_var_mapping (vars rΓ)  = Some ι1 ->
     get_this_var_mapping (vars rΓ') = Some ι2 ->
     ι1 = ι2.
@@ -1646,7 +1646,7 @@ Proof.
   intros CT sΓ rΓ h stmt sΓ' rΓ' h' ι1 ι2
          Hwf Htyp Heval Hthis1 Hthis2.
   pose proof (eval_stmt_preserves_receiver_addr_mapping_eq
-                CT sΓ rΓ h stmt sΓ' rΓ' h' Hwf Htyp Heval) as Heq.
+               CT sΓ rΓ h stmt sΓ' rΓ' h' Hwf Htyp Heval) as Heq.
   rewrite Hthis1 in Heq.
   rewrite Hthis2 in Heq.
   inversion Heq; reflexivity.
@@ -1655,7 +1655,7 @@ Qed.
 Lemma eval_stmt_preserves_receiver_r_type_typed :
   forall CT sΓ rΓ h stmt sΓ' rΓ' h' ι rqt,
     stmt_typing CT sΓ stmt sΓ' ->
-    eval_stmt OK CT rΓ h stmt OK rΓ' h' ->
+    eval_stmt OK (protected_locset_from_env CT h rΓ) CT rΓ h stmt OK (protected_locset_from_env CT h rΓ) rΓ' h' ->
     get_this_var_mapping (vars rΓ) = Some ι ->
     r_type h ι = Some rqt ->
     ι < dom h ->
@@ -1677,7 +1677,7 @@ Qed.
 Lemma eval_stmt_preserves_receiver_r_muttype_typed :
   forall CT sΓ rΓ h stmt sΓ' rΓ' h' ι q,
     stmt_typing CT sΓ stmt sΓ' ->
-    eval_stmt OK CT rΓ h stmt OK rΓ' h' ->
+    eval_stmt OK (protected_locset_from_env CT h rΓ) CT rΓ h stmt OK (protected_locset_from_env CT h rΓ) rΓ' h' ->
     get_this_var_mapping (vars rΓ) = Some ι ->
     r_muttype h ι = Some q ->
     ι < dom h ->
@@ -1698,7 +1698,7 @@ Qed.
 
 Lemma eval_stmt_preserves_r_type_backwards : 
   forall CT rΓ h stmt rΓ' h' loc rqt,
-    eval_stmt OK CT rΓ h stmt OK rΓ' h' ->
+    eval_stmt OK (protected_locset_from_env CT h rΓ) CT rΓ h stmt OK (protected_locset_from_env CT h rΓ) rΓ' h' ->
     r_type h' loc = Some rqt ->
     loc < dom h ->
     r_type h loc = Some rqt.
@@ -1724,7 +1724,7 @@ Lemma eval_stmt_preserves_receiver_r_type_typed_backwards :
   forall CT sΓ rΓ h stmt sΓ' rΓ' h' ι rqt,
     wf_r_config CT sΓ rΓ h ->
     stmt_typing CT sΓ stmt sΓ' ->
-    eval_stmt OK CT rΓ h stmt OK rΓ' h' ->
+    eval_stmt OK (protected_locset_from_env CT h rΓ) CT rΓ h stmt OK (protected_locset_from_env CT h rΓ) rΓ' h' ->
     get_this_var_mapping (vars rΓ') = Some ι ->
     r_type h' ι = Some rqt ->
     ι < dom h ->
@@ -1756,7 +1756,7 @@ Qed.
 
 Lemma eval_stmt_preserves_r_muttype_backwards : 
   forall CT rΓ h stmt rΓ' h' loc q,
-    eval_stmt OK CT rΓ h stmt OK rΓ' h' ->
+    eval_stmt OK (protected_locset_from_env CT h rΓ) CT rΓ h stmt OK (protected_locset_from_env CT h rΓ) rΓ' h' ->
     r_muttype h' loc = Some q ->
     loc < dom h ->
     r_muttype h loc = Some q.
@@ -1779,7 +1779,7 @@ Lemma eval_stmt_preserves_receiver_r_muttype_typed_backwards :
   forall CT sΓ rΓ h stmt sΓ' rΓ' h' ι q,
     wf_r_config CT sΓ rΓ h ->
     stmt_typing CT sΓ stmt sΓ' ->
-    eval_stmt OK CT rΓ h stmt OK rΓ' h' ->
+    eval_stmt OK (protected_locset_from_env CT h rΓ) CT rΓ h stmt OK (protected_locset_from_env CT h rΓ) rΓ' h' ->
     get_this_var_mapping (vars rΓ') = Some ι ->
     r_muttype h' ι = Some q ->
     ι < dom h ->
@@ -1933,15 +1933,15 @@ Proof.
 Qed.
 
 Lemma preservation_varass_ok :
-  forall CT sΓ rΓ h x e v2 sΓ',
+  forall P CT sΓ rΓ h x e v2 sΓ',
     OK = OK ->
     wf_r_config CT sΓ rΓ h ->
     stmt_typing CT sΓ (SVarAss x e) sΓ' ->
-    eval_expr OK CT rΓ h e v2 OK rΓ h ->
+    eval_expr OK P CT rΓ h e v2 OK P rΓ h ->
     runtime_getVal rΓ x <> None ->
     wf_r_config CT sΓ' (rΓ <| vars := update x v2 (vars rΓ) |>) h.
 Proof.
-    intros CT sΓ rΓ h x e v2 sΓ' HOK Hwf Htyping Heval Hruntime_getVal.
+    intros P CT sΓ rΓ h x e v2 sΓ' HOK Hwf Htyping Heval Hruntime_getVal.
     inversion Htyping; subst.
     have Hwfcopy := Hwf.
     revert Hwfcopy.
@@ -2087,7 +2087,7 @@ Proof.
           assert (H_loc_Te : wf_r_typable CT rΓ h loc Te qcontext).
           {
             (* Apply expression evaluation preservation lemma *)
-            apply (expr_eval_preservation CT sΓ' rΓ h e (Iot loc) rΓ h Te ι).
+            apply (expr_eval_preservation P CT sΓ' rΓ h e (Iot loc) rΓ h Te ι).
             auto.
             - rewrite get_this_var_mapping_update_vars_nonzero in HreceiverAddr. exact H4. exact HreceiverAddr.
             - exact Hreceivermut.
@@ -3481,7 +3481,7 @@ Theorem preservation_pico :
   forall CT sΓ rΓ h stmt rΓ' h' sΓ',
     wf_r_config CT sΓ rΓ h ->
     stmt_typing CT sΓ stmt sΓ' -> 
-    eval_stmt OK CT rΓ h stmt OK rΓ' h' -> 
+    eval_stmt OK (protected_locset_from_env CT h rΓ) CT rΓ h stmt OK (protected_locset_from_env CT h rΓ) rΓ' h' -> 
     wf_r_config CT sΓ' rΓ' h'.
 Proof.
   intros CT sΓ rΓ h stmt rΓ' h' sΓ' Hwf Htyping Heval.
