pico-invsubtyping-limitedvpa/Reachability.v
@@ -1,0 +1,64 @@
+From Stdlib Require Import Lia.
+Require Import List.
+Import ListNotations.
+Require Import Syntax Typing Subtyping ViewpointAdaptation Helpers.
+Require Import String.
+Require Import Stdlib.Sets.Ensembles.
+From RecordUpdate Require Import RecordUpdate.
+Require Import Stdlib.Logic.Classical_Prop.
+Require Import Stdlib.Classes.RelationClasses.
+
+Inductive reachable (h : heap): Loc -> Loc -> Prop :=
+
+| rch_heap:
+    forall l,
+      l < dom h ->
+      reachable h l l
+
+| rch_step:
+    forall l0 l1 obj f,
+      l1 < dom h ->
+      runtime_getObj h l0 = Some obj ->
+      getVal obj.(fields_map) f = Some (Iot l1) ->
+      reachable h l0 l1
+
+| rch_trans:
+    forall l0 l1 l2,
+      reachable h l0 l1 ->
+      reachable h l1 l2 ->
+      reachable h l0 l2.
+
+
+Inductive reachable_abs (CT : class_table) (h : heap) : Loc -> Loc -> Prop :=
+
+| reachable_abs_heap :
+    forall l,
+      l < dom h ->
+      reachable_abs CT h l l
+
+| reachable_abs_step :
+    forall l0 l1 any C vals k,
+      (* concrete step, as in [rch_step] *)
+      l1 < dom h ->
+      runtime_getObj h l0 = Some (mkObj (mkruntime_type any C) vals) ->
+      (* field [f] corresponds to index [k] and is RDM/Imm in the abstract state *)
+      nth_error vals k = Some (Iot l1) ->
+      (sf_mutability_rel CT C k RDM_f \/
+       sf_mutability_rel CT C k Imm_f) ->
+      (sf_assignability_rel CT C k RDA \/
+      sf_assignability_rel CT C k Final) ->
+      reachable_abs CT h l0 l1
+
+| reachable_abs_trans :
+    forall l0 l1 l2,
+      reachable_abs CT h l0 l1 ->
+      reachable_abs CT h l1 l2 ->
+      reachable_abs CT h l0 l2.
+
+Definition reachable_locset
+           (CT : class_table) (h : heap) (root : Loc) : Ensembles.Ensemble Loc :=
+  fun l => reachable_abs CT h root l.
+
+Definition protected_locset
+  (CT : class_table) (h : heap) (l_root : Loc) : Ensembles.Ensemble Loc :=
+  fun l_target => reachable_abs CT h l_root l_target.
